src/high/no_buffer.v
@@ -1,0 +1,105 @@
+From iris.proofmode Require Import tactics.
+From iris.bi Require Import bi.
+From iris.bi Require Import derived_laws.
+
+From self.high Require Import dprop resources crash_weakestpre weakestpre
+     recovery_weakestpre resources lifted_modalities modalities post_crash_modality protocol.
+
+Class IntoNoBuffer {Σ} (P : dProp Σ) (Q : dProp Σ) :=
+  into_no_buffer : P ⊢ <nobuf> Q.
+Global Arguments IntoNoBuffer {_} _%I _%I.
+Global Arguments into_no_buffer {_} _%I _%I {_}.
+Global Hint Mode IntoNoBuffer + ! -  : typeclass_instances.
+
+Ltac iModel := iStartProof (iProp _); iIntros (TV).
+
+Section no_buffer.
+  Context `{Σ : gFunctors}.
+  Implicit Types (P : dProp Σ).
+
+
+  Lemma no_buff_at_alt P SV PV BV : ((<nobuf> P) (SV, PV, BV) = P (SV, PV, ∅))%I.
+  Proof. done. Qed.
+
+  Lemma no_buffer_at P TV : ((<nobuf> P) TV = P (store_view TV, flush_view TV, ∅))%I.
+  Proof. destruct TV as [[??]?]. apply no_buff_at_alt. Qed.
+
+  Lemma no_buffer_pure φ : ⌜φ⌝ -∗ <nobuf> (⌜φ⌝ : dProp Σ).
+  Proof. iModel. by rewrite no_buffer_at monPred_at_pure. Qed.
+
+  Lemma no_buffer_embed (P : iProp Σ) : ⎡P⎤ -∗ <nobuf> (⎡P⎤ : dProp Σ).
+  Proof. iModel. rewrite no_buffer_at monPred_at_embed. naive_solver. Qed.
+
+  Lemma no_buffer_mono P Q : (P ⊢ Q) → <nobuf> P ⊢ <nobuf> Q.
+  Proof. intros H. iModel. rewrite 2!no_buffer_at. iApply H. Qed.
+
+  Lemma no_buffer_emp : (emp : dProp Σ) ⊢ <nobuf> emp.
+  Proof. iModel. by rewrite no_buffer_at monPred_at_emp. Qed.
+
+  Lemma no_buffer_and P Q : <nobuf> (P ∧ Q) ⊣⊢ <nobuf> P ∧ <nobuf> Q.
+  Proof. iModel. rewrite !no_buffer_at. rewrite monPred_at_and. naive_solver. Qed.
+
+  Lemma no_buffer_sep P Q : <nobuf> (P ∗ Q) ⊣⊢ <nobuf> P ∗ <nobuf> Q.
+  Proof. iModel. rewrite !no_buffer_at. rewrite monPred_at_sep. naive_solver. Qed.
+
+  Lemma no_buffer_intuitionistically_2 P : □ <nobuf> P ⊢ <nobuf> □ P.
+  Proof.
+    iModel. rewrite !no_buffer_at monPred_at_intuitionistically. naive_solver.
+  Qed.
+
+  Lemma modality_no_buffer_mixin :
+    modality_mixin (@no_buffer Σ)
+      (MIEnvTransform IntoNoBuffer) (MIEnvTransform IntoNoBuffer).
+  Proof.
+    split; simpl; split_and?;
+    eauto using bi.equiv_entails_1_2, no_buffer_and, no_buffer_emp,
+      no_buffer_mono, no_buffer_sep.
+    intros P Q. rewrite /IntoNoBuffer=> ->.
+    by rewrite no_buffer_intuitionistically_2.
+  Qed.
+  Definition modality_no_buffer :=
+    Modality _ modality_no_buffer_mixin.
+
+  (* Lemma no_buffer_know_protocol ϕ *)
+  (*   know_flush_lb ℓa n -∗  *)
+
+  Global Instance from_modal_no_buffer P :
+    FromModal True (modality_no_buffer) (<nobuf> P) (<nobuf> P) P.
+  Proof. by rewrite /FromModal. Qed.
+
+  Global Instance into_no_buffer_pure φ : IntoNoBuffer (⌜φ⌝ : dProp Σ)%I ⌜φ⌝.
+  Proof. rewrite /IntoNoBuffer. eauto using no_buffer_pure. Qed.
+
+  Global Instance into_no_buffer_embed (P : iProp Σ) : IntoNoBuffer ⎡P⎤ ⎡P⎤.
+  Proof. rewrite /IntoNoBuffer. eauto using no_buffer_embed. Qed.
+
+End no_buffer.
+
+Section no_buffer_rules.
+  (* Some less "basic" rules for <nobuf>. *)
+  Context `{nvmFixedG Σ, hGD : nvmDeltaG Σ}.
+
+  Lemma no_buffer_know_flush_lb `{AbstractState ST} ℓ (s : ST) :
+    know_flush_lb ℓ s -∗ <nobuf> know_flush_lb ℓ s.
+  Proof.
+  Admitted.
+  (*   rewrite /know_flush_lb. *)
+  (*   iModel. *)
+  (*   simpl. *)
+  (* Qed. *)
+End no_buffer_rules.
+
+Section no_buffer_test.
+
+  Context `{Σ : gFunctors}.
+  Implicit Types (P : dProp Σ).
+
+  Lemma test φ (P : iProp Σ) :
+    ⌜φ⌝ -∗ ⎡P⎤ -∗ <nobuf> (⌜φ⌝ ∗ ⎡P⎤).
+  Proof.
+    iIntros "ph P".
+    iModIntro.
+    iFrame.
+  Qed.
+
+End no_buffer_test.
